IP Header example done, modulo some proofs.

src/Narcissus/Examples/NetworkStack/IPv4Header.v
@@ -18,10 +18,10 @@ Require Import
         Fiat.Narcissus.Common.ComposeCheckSum
         Fiat.Narcissus.Common.ComposeIf
         Fiat.Narcissus.Common.ComposeOpt
-        Fiat.Narcissus.Automation.Solver
-        Fiat.Narcissus.Automation.AlignedAutomation
         Fiat.Narcissus.Formats
-        Fiat.Narcissus.Stores.EmptyStore.
+        Fiat.Narcissus.Stores.EmptyStore
+        Fiat.Narcissus.Automation.Solver
+        Fiat.Narcissus.Automation.AlignedAutomation.
 
 Require Import Bedrock.Word.
 
@@ -30,8 +30,18 @@ Open Scope string_scope.
 Open Scope Tuple_scope.
 
 (* Our source data type for IP packets. *)
-Definition IPv4_Packet :=
-  @Tuple <"TotalLength" :: word 16,
+Record IPv4_Packet :=
+  { TotalLength : word 16;
+     ID : word 16;
+     DF : bool; (* Don't fragment flag *)
+     MF : bool; (*  Multiple fragments flag *)
+     FragmentOffset : word 13;
+     TTL : word 8;
+     Protocol : EnumType ["ICMP"; "TCP"; "UDP"];
+     SourceAddress : word 32;
+     DestAddress : word 32;
+     Options : list (word 32) }.
+(*@Tuple <"TotalLength" :: word 16,
   "ID" :: word 16,
   "DF" :: bool, (* Don't fragment flag *)
   "MF" :: bool, (*  Multiple fragments flag *)
@@ -40,7 +50,7 @@ Definition IPv4_Packet :=
   "Protocol" :: EnumType ["ICMP"; "TCP"; "UDP"],
   "SourceAddress" :: word 32,
   "DestAddress" :: word 32,
-  "Options" :: list (word 32)>.
+  "Options" :: list (word 32)>.*)
 
 (* Protocol Numbers from [RFC5237]*)
 Definition ProtocolTypeCodes : Vector.t (word 8) 3 :=
@@ -49,30 +59,30 @@ Definition ProtocolTypeCodes : Vector.t (word 8) 3 :=
      WO~0~0~0~1~0~0~0~1  (* UDP:  17*)
   ].
 
-Definition IPv4_Packet_Header_Len (ip4 : IPv4_Packet) := 5 + |ip4!"Options"|.
+Definition IPv4_Packet_Header_Len (ip4 : IPv4_Packet) := 5 + |ip4.(Options)|.
 
 Definition IPv4_Packet_Format (ip4 : IPv4_Packet)  :=
   (format_word (natToWord 4 4)
                ThenC format_nat 4 (IPv4_Packet_Header_Len ip4)
                ThenC format_unused_word 8 (* TOS Field! *)
-               ThenC format_word ip4!"TotalLength"
-               ThenC format_word ip4!"ID"
+               ThenC format_word ip4.(TotalLength)
+               ThenC format_word ip4.(ID)
                ThenC format_unused_word 1 (* Unused flag! *)
-               ThenC format_bool ip4!"DF"
-               ThenC format_bool ip4!"MF"
-               ThenC format_word ip4!"FragmentOffset"
-               ThenC format_word ip4!"TTL"
-               ThenC format_enum ProtocolTypeCodes ip4!"Protocol"
+               ThenC format_bool ip4.(DF)
+               ThenC format_bool ip4.(MF)
+               ThenC format_word ip4.(FragmentOffset)
+               ThenC format_word ip4.(TTL)
+               ThenC format_enum ProtocolTypeCodes ip4.(Protocol)
                DoneC)
     ThenChecksum IPChecksum_Valid' OfSize 16
-    ThenCarryOn (format_word ip4!"SourceAddress"
-                             ThenC format_word ip4!"DestAddress"
-                             ThenC format_list format_word ip4!"Options"
+    ThenCarryOn (format_word ip4.(SourceAddress)
+                             ThenC format_word ip4.(DestAddress)
+                             ThenC format_list format_word ip4.(Options)
                              DoneC)%format.
 
 Definition IPv4_Packet_OK (ipv4 : IPv4_Packet) :=
-  lt (|ipv4!"Options"|) 11 /\
-  lt (20 + 4 * |ipv4!"Options"|) (wordToNat ipv4!"TotalLength").
+  lt (|ipv4.(Options)|) 11 /\
+  lt (20 + 4 * |ipv4.(Options)|) (wordToNat ipv4.(TotalLength)).
 
 (* Step One: Synthesize an encoder and a proof that it is correct. *)
 
@@ -87,84 +97,49 @@ Defined.
 Definition ipv4_encoder_impl r {sz} v :=
   Eval simpl in (projT1 ipv4_encoder r sz v 0 tt).
 
+(* Step Two and a Half: Add some simple facts about correct packets
+   for the decoder automation. *)
 Lemma IPv4_Packet_Header_Len_eq
-  : forall data len,
-    IPv4_Packet_Header_Len data = len
-    -> ((|data!"Options" |) = len - 5).
+  : forall packet len,
+    IPv4_Packet_Header_Len packet = len
+    -> ((|packet.(Options) |) = len - 5).
 Proof.
   unfold IPv4_Packet_Header_Len; intros.
   apply Minus.plus_minus.
   rewrite H; reflexivity.
 Qed.
 
+Lemma IPv4_Packet_Header_Len_bound
+  : forall packet,
+    IPv4_Packet_OK packet ->
+    lt (IPv4_Packet_Header_Len packet) (pow2 4)%nat.
+Proof.
+  intros; replace (pow2 4) with 16 by reflexivity.
+  unfold IPv4_Packet_OK in H; unfold IPv4_Packet_Header_Len.
+  omega.
+Qed.
+
 Hint Resolve IPv4_Packet_Header_Len_eq : data_inv_hints.
+Hint Resolve IPv4_Packet_Header_Len_bound : data_inv_hints.
 
-Arguments wordToNat : simpl never.
-
-Definition EthernetHeader_decoder
+(* Step Three: Synthesize a decoder and a proof that /it/ is correct. *)
+Definition IPv4_Packet_Header_decoder
   : CorrectAlignedDecoderFor IPv4_Packet_OK IPv4_Packet_Format.
 Proof.
   eapply CorrectAlignedDecoderForIPChecksumThenC.
   cbv beta; unfold Domain; simpl; repeat calculate_length_ByteString.
-  unfold IPv4_Packet_OK.
   start_synthesizing_decoder.
   normalize_compose AlignedByteString.ByteStringQueueMonoid.
-  decode_step idtac.
-  decode_step idtac.
-  decode_step idtac.
-  decode_step idtac.
-  decode_step idtac.
-  decode_step idtac.
-  decode_step idtac.
-  admit.
-  repeat decode_step idtac.
   repeat decode_step idtac.
   cbv beta; synthesize_cache_invariant.
   cbv beta; unfold decode_nat; optimize_decoder_impl.
-  eapply @AlignedDecoders.AlignedDecode_Sumb.
-  eapply @AlignedDecode_CollapseWord; eauto.
-  eapply @AlignedDecodeBindCharM; intros.
-  intros; apply @AlignedDecode_Sumb.
-  eapply @AlignedDecodeBindUnusedCharM; simpl;
-    eapply DecodeMEquivAlignedDecodeM_trans;
-      [ | intros; reflexivity
-        |  ].
-  eapply @AlignedDecodeBind2CharM; intros; eauto.
-  eapply @AlignedDecodeBind2CharM; intros; eauto.
-  eapply @AlignedDecoders.AlignedDecode_Sumb.
-  eapply AlignedDecode_CollapseWord';
-    eauto using decode_word_eq_decode_unused_word,
-    decode_word_eq_decode_bool,
-    decode_word_eq_decode_word.
-  eapply @AlignedDecoders.AlignedDecode_Sumb.
-  eapply AlignedDecode_CollapseWord';
-    eauto using decode_word_eq_decode_unused_word,
-    decode_word_eq_decode_bool,
-    decode_word_eq_decode_word.
-  eapply @AlignedDecoders.AlignedDecode_Sumb.
-  eapply AlignedDecode_CollapseWord';
-    eauto using decode_word_eq_decode_unused_word,
-    decode_word_eq_decode_bool,
-    decode_word_eq_decode_word.
-  eapply @AlignedDecodeBind2CharM; intros; eauto.
-  eapply @AlignedDecodeBindCharM; intros; eauto.
-  eapply @AlignedDecodeBindEnumM; intros; eauto.
-  eapply @AlignedDecodeBindUnused2CharM; simpl;
-    eapply DecodeMEquivAlignedDecodeM_trans;
-      [ | intros; reflexivity
-        |  ].
-  eapply @AlignedDecodeBind4CharM; intros; eauto.
-  eapply @AlignedDecodeBind4CharM; intros; eauto.
-  eapply @AlignedDecodeListM; intros; eauto.
-  eapply (fun H H' => @AlignedDecodeNCharM _ _ H H' 4); eauto; simpl; intros.
-  eapply @AlignedDecode_ifb.
-  eapply @Return_DecodeMEquivAlignedDecodeM.
-  intros; higher_order_reflexivity.
-  intros; higher_order_reflexivity.
+  repeat align_decoders_step.
 Defined.
 
+(* Step Four: Extract the decoder function, and have /it/ start decoding
+   at the start of the provided ByteString [v]. *)
 Definition IPv4_decoder_impl {sz} v :=
-  Eval simpl in (projT1 EthernetHeader_decoder sz v 0 ()).
+  Eval simpl in (projT1 IPv4_Packet_Header_decoder sz v 0 ()).
 
 Definition pkt' : Vector.t (word 8) _ :=
   [WO~1~0~1~0~0~0~1~0;
